proof_of_soundness/Theorems.v
@@ -11,8 +11,6 @@ From Cpp2C Require Import Transformations.
 
 Open Scope string_scope.
 
-Section Theorems.
-
 (* A constant macro is the same as a constant function with the same return
    expression *)
 Lemma constant_function_macro_eq_to_function :
@@ -61,134 +59,112 @@ Proof.
 Qed.
 
 
-(* An expressions evaluates to the same value under an expanded
-   function definition list *)
-Theorem evaluation_eq_under_expanded_func_list :
-  forall S E F M e v S' F',
-  exprevalR S E F M e v S' = exprevalR S E F' M e v S'.
-Proof.
-Admitted.
-
-
-Theorem macro_transformation_sound :
-  forall (S S': state) (E : environment)
-         (F F': func_definitions) (M M': macro_definitions)
-         (e e' mexpr: expr) (mname fname: string)
-         (v : Z),
-  definition mname F = None ->
-  invocation mname M = Some mexpr ->
-  has_side_effects mexpr = false ->
-  get_dynamic_vars mexpr = nil ->
+(* We currently need this theorem for the soundndess proof.
+   It basically says that if an expression could be evaluated under the
+   original function list, it can be evaluated correctly under the
+   transformed function list as well. We know this will be true in
+   the implementation since we will guarantee that all the function
+   names will be unique, but we need this for the proof. *)
+Lemma eval_same_under_unique_names :
+  forall S E F M v S' x mexpr,
   exprevalR S E F M mexpr v S' ->
-  e = CallOrInvocation mname ->
-  (F', M', e') = transform_macros F M e ->
-  exprevalR S E F M e v S' <-> exprevalR S E F' M' e' v S'.
-Proof.
-  intros. unfold transform_macros in H5.
-  rewrite H4, H, H0, H1, H2 in H5. simpl in H5.
-  inversion H5.
-  split.
-  - intros.
-     + apply E_FunctionCall with (fstmt:=Skip) (fexpr:=mexpr) (S':=S).
-      * unfold definition. simpl.
-        rewrite eqb_refl. simpl. reflexivity.
-      * apply E_Skip.
-      * rewrite evaluation_eq_under_expanded_func_list with (F':=F).
-        apply H3.
-  - intros. rewrite H4. apply E_MacroInvocation with (mexpr := mexpr).
-    + apply H0.
-    + apply H3.
-Qed.
-
-Theorem foo: forall F M e e' F' M',
-  transform_macros F M e = (F', M', e') ->
-  transform_macros F M (ParenExpr e) = (F', M', ParenExpr e').
-Proof.
-  intros. unfold transform_macros.
+  exprevalR S E ((x ++ "__as_function", (Skip, mexpr)) :: F) M mexpr v S'.
 Admitted.
 
-Theorem bar: forall F M e e' F' M' F'' M'',
-  transform_macros F M (ParenExpr e) = (F', M', ParenExpr e') ->
-  transform_macros F M e = (F'', M'', e') ->
-  (F', M') = (F'', M'').
-Proof.
-  intros. simpl in H. rewrite H0 in H.
-  inversion H.
-  reflexivity.
-Qed.
 
-Theorem lookup_eq :
-  forall S E F M x F' M' S' v0 v1,
-  exprevalR S E F M (X x) v0 S' ->
-  exprevalR S E F' M' (X x) v1 S' ->
-  v0 = v1.
-Proof.
-Admitted.
-
-Theorem paren_no_paren_eq :
-  forall S E F M pe0 pe1  S' pv0 pv1,
-  exprevalR S E F M pe0 pv0 S' ->
-  exprevalR S E F M pe1 pv1 S' ->
-  pv0 = pv1.
+Theorem transform_macros_sound :
+  forall S E F M e v S',
+  exprevalR S E F M e v S' ->
+  exprevalR S E (transform_macros_F F M e) (transform_macros_M F M e) (transform_macros_e F M e) v S'.
 Proof.
   intros.
-Admitted.
-
-
-Theorem macro_transformation_sound_all :
-  forall (S S': state) (E : environment)
-         (F F': func_definitions) (M M': macro_definitions)
-         (e e' e'' mexpr: expr) (mname fname: string)
-         (v0 v1 : Z),
-  transform_macros F M e = (F', M', e') ->
-  exprevalR S E F M e v0 S' ->
-  exprevalR S E F' M' e' v1 S' ->
-  v0 = v1.
-Proof.
-  intros. induction e.
-  - inversion H. inversion H0. rewrite <- H9.
-    inversion H. rewrite <- H5 in H1. inversion H1.
-    reflexivity.
-  - inversion H. rewrite <- H5 in H1.
-    eapply lookup_eq.
+  induction H; unfold transform_macros_M in *.
+  - (* Num z *)
+    apply E_Num.
+  - (* X x *)
+    apply E_X_Success with l.
+    + apply H.
     + apply H0.
-    + apply H1.
-  - eapply bar in H.
-    + inversion H. apply IHe.
-      * rewrite H3. rewrite H4.
+  - (* ParenExpr e *)
+    apply E_ParenExpr. apply IHexprevalR.
+  - (* UnExpr uo e *)
+    apply E_UnExpr. apply IHexprevalR.
+  - (* BinExpr bo e1 e2 *)
+    apply E_BinExpr with (S:=S) (S':=S').
+    + fold transform_macros_e. admit.
+    + fold transform_macros_e. admit.
+  - (* Assign x e *)
+    apply E_Assign_Success. apply IHexprevalR. apply H0.
+  - (* CallOrInvocation x (function call) *)
+    unfold transform_macros_F. unfold transform_macros_e.
+    rewrite H. apply E_FunctionCall with (fstmt:=fstmt) (fexpr:=fexpr)
+    (S':=S'). apply H. apply H0. apply H1.
+  - (* CallOrInvocation x (macro invocation) *)
+    unfold transform_macros_F.
+    unfold transform_macros_e.
+    rewrite H.
+    destruct (definition x F).
+    + (* x is defined as a function
+      (shouldn't happen so just use E_MacroInvocation *)
+      apply E_MacroInvocation with mexpr. apply H. apply H0.
+    + (* x is not defined as a function *)
+      destruct (has_side_effects mexpr).
+      * (* x's body has side-effects *)
+        destruct (get_dynamic_vars mexpr).
+           (* x does not have side-effects (does nothing) *)
+        -- apply E_MacroInvocation with mexpr. apply H. apply H0.
+           (* x  has side-effects (does nothing) *)
+        -- apply E_MacroInvocation with mexpr. apply H. apply H0.
+      * destruct (get_dynamic_vars mexpr).
+           (* x does not share variables with the caller environment.
+              Here is where we perform the simplest transformation. *)
+        -- apply E_FunctionCall with (fstmt:=Skip) (fexpr:=mexpr) (S':=S).
+           ++ unfold definition. unfold find.
+              simpl. rewrite eqb_refl. auto.
+           ++ apply E_Skip.
+              (* Here is where we need a lemma stating that
+                 under the new function list, the evaluation of the
+                 transformed macro body will be the same.
+                 Intuitively we know this will be true since all
+                 the names in the transformed function list will be
+                 unique, and we will only add names, never remove any. *)
+           ++ apply eval_same_under_unique_names. apply H0.
+           (* x shares variables with the caller environment *)
+        -- apply E_MacroInvocation with mexpr. apply H. apply H0.
 Admitted.
+
+
+(* Expression evaluation does not change under the ID transformation *)
+Theorem transform_id_sound :
+  forall S E F M e v S',
+  exprevalR S E F M e v S' ->
+  exprevalR S E F M (transform_id e) v S'.
+Proof.
+  intros.
+  induction H.
+  - (* Num z *)
+    apply E_Num.
+  - (* X x *)
+    apply E_X_Success with l. apply H. apply H0.
+  - (* ParenExpr e *)
+    constructor. apply IHexprevalR.
+  - (* UnExpr uo e *)
+    constructor. apply IHexprevalR.
+  - (* BinExpr bo e1 e2 *)
+    apply E_BinExpr with (S:=S) (S':=S').
+    apply IHexprevalR1. apply IHexprevalR2.
+  - (* Assign x e *)
+    constructor. apply IHexprevalR. apply H0.
+  - (* CallOrInvocation x (function call) *)
+    apply E_FunctionCall with (fstmt:=fstmt) (fexpr:=fexpr) (S':=S').
+    apply H. apply H0. apply H1.
+  - (* CallOrInvocation x (macro invocation) *)
+   apply E_MacroInvocation with mexpr. apply H. apply H0.
+Qed.
 
 
 (* NOTE: May want to note in paper that we have to transform
          function and macro arguments recursively *)
-(* TODO: Create a funtion that does an identity transform,
-         then create a theorem that proves by induction
-         that untransformed and transformed programs are
-         identical *)
-
-Theorem transform_id_eq :
-  forall e,
-  e = transform_id e.
-Proof.
-  intros.
-  induction e.
-  - reflexivity.
-  - reflexivity.
-  - simpl. rewrite <- IHe. reflexivity.
-  - simpl. rewrite <- IHe. reflexivity.
-  - simpl. rewrite <- IHe1. rewrite <- IHe2. reflexivity.
-  - simpl. rewrite <- IHe. reflexivity.
-  - reflexivity.
-Qed.
-
-Theorem id_args_eq : forall (args : list expr),
-  args = map transform_id args.
-Proof.
-  intros.
-  induction args.
-  - reflexivity.
-  - simpl. rewrite <- transform_id_eq. rewrite <- IHargs. reflexivity.
-Qed.
 
 (* We may need three separate theorems, proving
    1) Equivalence under expression transformation
@@ -198,6 +174,5 @@ Qed.
    that the other two transformations are sound
 *)
 
-End Theorems.
 
 Close Scope string_scope.
